Start propagating uint64-ness

lib/Lang/LinearSequence.i.dfy
@@ -54,7 +54,7 @@ module LinearSequence_i {
   function lseqs<A>(l:lseq<A>):(s:seq<A>)
     ensures rank_is_less_than(s, l)
   {
-    var s := seq(lseq_length_raw(l), i requires 0<=i<lseq_length_raw(l) => read(lseqs_raw(l)[i]));
+    var s := seq(lseq_length_raw(l), (i:int) requires 0<=i<lseq_length_raw(l) as int => read(lseqs_raw(l)[i]));
     axiom_lseqs_rank(l, s);
     s
   }
@@ -80,7 +80,7 @@ module LinearSequence_i {
   function lseq_has<A>(l:lseq<A>):(s:seq<bool>)
       ensures |s| == |lseqs(l)|
   {
-      seq(lseq_length_raw(l), i requires 0<=i<lseq_length_raw(l) => has(lseqs_raw(l)[i]))
+      seq(lseq_length_raw(l), (i:int) requires 0<=i<lseq_length_raw(l) as int => has(lseqs_raw(l)[i]))
   }
 
   predicate lseq_has_all<A>(l:lseq<A>)
@@ -88,89 +88,89 @@ module LinearSequence_i {
     forall i :: 0<=i<|l| ==> lseq_has(l)[i]
   }
 
-  function method lseq_length<A>(shared s:lseq<A>):(n:nat)
-      ensures n == |lseqs(s)|
+  function method lseq_length<A>(shared s:lseq<A>):(n:uint64)
+      ensures n as int == |lseqs(s)|
   {
       lseq_length_raw(s)
   }
 
-  function method{:inline true} operator(| |)<A>(shared s:seq<A>):nat
+  function method{:inline true} operator(| |)<A>(shared s:seq<A>):uint64
   {
       seq_length(s)
   }
 
-  function method{:inline true} operator(| |)<A>(shared s:lseq<A>):nat
+  function method{:inline true} operator(| |)<A>(shared s:lseq<A>):uint64
   {
       lseq_length(s)
   }
 
-  function{:inline true} operator([])<A>(s:lseq<A>, i:nat):A
+  function{:inline true} operator([])<A>(s:lseq<A>, i:uint64):A
       requires i < |s|
   {
       lseqs(s)[i]
   }
 
-  function{:inline true} operator(in)<A>(s:lseq<A>, i:nat):bool
-      requires i < |s|
+  function{:inline true} operator(in)<A>(s:lseq<A>, i:uint64):bool
+      requires i as int < |s| as int
   {
       lseq_has(s)[i]
   }
 
   function method lseq_peek<A>(shared s:lseq<A>, i:uint64):(shared a:A)
-      requires i as nat < |s| && i as nat in s
-      ensures a == s[i as nat]
+      requires i as nat < |s| as nat && i in s
+      ensures a == s[i]
   {
       peek(lseq_share_raw(s, i))
   }
 
   method lseq_alloc<A>(length:uint64) returns(linear s:lseq<A>)
-      ensures |s| == length as nat
-      ensures forall i:nat | i < length as nat :: i !in s
+      ensures |s| == length
+      ensures forall i | i < length :: i !in s
   {
       s := lseq_alloc_raw(length);
   }
 
   method lseq_free<A>(linear s:lseq<A>)
-      requires forall i:nat | i < |s| :: i !in s
+      requires forall i | i < |s| :: i !in s
   {
-      assert forall i:nat {:trigger lseqs_raw(s)[i]} | i < |lseqs_raw(s)| :: i !in s;
+      assert forall i:uint64 {:trigger lseqs_raw(s)[i]} | i as int < |lseqs_raw(s)| :: i !in s;
       var _ := lseq_free_raw(s);
   }
 
   // can be implemented as in-place swap
   method lseq_swap<A>(linear s1:lseq<A>, i:uint64, linear a1:A) returns(linear s2:lseq<A>, linear a2:A)
-      requires i as nat < |s1| && i as nat in s1
-      ensures a2 == s1[i as nat]
+      requires i < |s1| && i in s1
+      ensures a2 == s1[i]
       ensures lseq_has(s2) == lseq_has(s1)
       ensures lseqs(s2) == lseqs(s1)[i as nat := a1]
   {
       linear var x1:maybe<A> := give(a1);
-      linear var x2:maybe<A>;
-      s2, x2 := lseq_swap_raw(s1, i, x1);
+      linear var (s2', x2) := lseq_swap_raw_fun(s1, i, x1);
+      s2 := s2';
       a2 := unwrap(x2);
   }
 
   method lseq_take<A>(linear s1:lseq<A>, i:uint64) returns(linear s2:lseq<A>, linear a:A)
-      requires i as nat < |s1| && i as nat in s1
-      ensures a == s1[i as nat]
+      requires i < |s1| && i in s1
+      ensures a == s1[i]
       ensures lseq_has(s2) == lseq_has(s1)[i as nat := false]
-      ensures forall j:nat | j < |s1| && j != i as nat :: lseqs(s2)[j] == lseqs(s1)[j]
+      ensures forall j:uint64 | j < |s1| && j != i :: lseqs(s2)[j] == lseqs(s1)[j]
   {
       linear var x1:maybe<A> := empty();
-      linear var x2:maybe<A>;
-      s2, x2 := lseq_swap_raw(s1, i, x1);
+      linear var (s2', x2) := lseq_swap_raw_fun(s1, i, x1);
+      s2 := s2';
       a := unwrap(x2);
   }
 
   method lseq_give<A>(linear s1:lseq<A>, i:uint64, linear a:A) returns(linear s2:lseq<A>)
-      requires i as nat < |s1|
-      requires i as nat !in s1
+      requires i < |s1|
+      requires i !in s1
       ensures lseq_has(s2) == lseq_has(s1)[i as nat := true]
       ensures lseqs(s2) == lseqs(s1)[i as nat := a]
   {
       linear var x1:maybe<A> := give(a);
-      linear var x2:maybe<A>;
-      s2, x2 := lseq_swap_raw(s1, i, x1);
+      linear var (s2', x2) := lseq_swap_raw_fun(s1, i, x1);
+      s2 := s2';
       var _ := discard(x2);
   }
 
@@ -200,31 +200,31 @@ module LinearSequence_i {
 
   method AllocAndMoveLseq<A>(linear source: lseq<A>, from: uint64, to: uint64)
     returns (linear looted: lseq<A>, linear loot: lseq<A>)
-    requires 0 <= from as nat <= to as nat <= |source|
-    requires forall j :: from as nat <= j < to as nat ==> j in source
+    requires 0 <= from <= to <= |source|
+    requires forall j :: from <= j < to ==> j in source
     ensures lseq_has_all(loot)
     ensures lseqs(loot) == lseqs(source)[from..to]
     ensures |looted| == |source|
-    ensures forall j :: 0<=j<|source| && !(from as nat <= j < to as nat) ==> looted[j] == old(source)[j]
+    ensures forall j :: 0<=j<|source| && !(from <= j < to) ==> looted[j] == old(source)[j]
     ensures forall j :: 0<=j<|source|
-      ==> lseq_has(looted)[j] == if from as nat <= j < to as nat then false else lseq_has(source)[j]
+      ==> lseq_has(looted)[j] == if from <= j < to then false else lseq_has(source)[j]
   {
     looted := source;
     ghost var count := (to - from) as nat;
     loot := lseq_alloc(to - from);
     var i:uint64 := from;
-    assert to as nat <= |old(source)|;
+    assert to <= |old(source)|;
     while i < to
       invariant from <= i <= to
-      invariant |loot| == count
-      invariant to as nat <= |looted|
+      invariant |loot| as nat == count
+      invariant to <= |looted|
       invariant forall j :: i <= j < to ==> lseq_has(looted)[j]
       invariant forall j :: 0 <= j < to-from ==> lseq_has(loot)[j] == (j < i-from)
       invariant lseqs(loot)[..i-from] == lseqs(old(source))[from..i]
       invariant |looted| == |old(source)|
-      invariant forall j :: 0<=j<|source| && !(from as nat <= j < i as nat) ==> looted[j] == old(source)[j]
+      invariant forall j :: 0<=j<|source| && !(from <= j < i) ==> looted[j] == old(source)[j]
       invariant forall j :: 0<=j<|looted|
-      ==> lseq_has(looted)[j] == if from as nat <= j < i as nat then false else lseq_has(old(source))[j]
+      ==> lseq_has(looted)[j] == if from <= j < i then false else lseq_has(old(source))[j]
     {
       linear var elt:A;
       looted, elt := lseq_take(looted, i);
@@ -240,17 +240,17 @@ module LinearSequence_i {
 
   method TrustedRuntimeLSeqResize<A>(linear s: lseq<A>, newlen: uint64)
     returns (linear s2: lseq<A>)
-    ensures |s2| == newlen as nat
-    ensures forall j :: 0 <= j < newlen as nat && j < |s| ==> lseq_has(s2)[j] == lseq_has(s)[j]
-    ensures forall j :: |s| <= j < newlen as nat ==> lseq_has(s2)[j] == false
-    ensures forall j :: 0 <= j < newlen as nat && j < |s| ==> s2[j] == s[j]
+    ensures |s2| == newlen 
+    ensures forall j :: 0 <= j < newlen && j < |s| ==> lseq_has(s2)[j] == lseq_has(s)[j]
+    ensures forall j :: |s| <= j < newlen ==> lseq_has(s2)[j] == false
+    ensures forall j :: 0 <= j < newlen && j < |s| ==> s2[j] == s[j]
 
   method InsertSeq<A>(linear s: seq<A>, a: A, pos: uint64) returns (linear s2: seq<A>)
     requires |s| < Uint64UpperBound() - 1;
     requires 0 <= pos as int <= |s|;
     ensures s2 == s[..pos] + [a] + s[pos..];
   {
-    var newlen: uint64 := seq_length(s) as uint64 + 1;
+    var newlen: uint64 := seq_length(s) + 1;
     s2 := TrustedRuntimeSeqResize(s, newlen);
 
     var i:uint64 := newlen - 1;
@@ -269,8 +269,8 @@ module LinearSequence_i {
 
   method InsertLSeq<A>(linear s: lseq<A>, linear a: A, pos: uint64) returns (linear s2: lseq<A>)
     requires lseq_has_all(s)  // robj points out that you only really need to has all the elements >=pos
-    requires |s| < Uint64UpperBound() - 1;
-    requires 0 <= pos as int <= |s|;
+    requires |s| as nat < Uint64UpperBound() - 1;
+    requires 0 <= pos <= |s|;
     ensures lseq_has_all(s2)
     ensures lseqs(s2) == lseqs(s)[..pos] + [a] + lseqs(s)[pos..];
   {
@@ -281,13 +281,13 @@ module LinearSequence_i {
     var i:uint64 := newlen - 1;
     while i > pos
       invariant i >= pos
-      invariant |s2| == newlen as nat;
+      invariant |s2| == newlen;
       // i is where we're writing next; it's the only hole in s2:
-      invariant forall j :: 0 <= j < |s2| ==> lseq_has(s2)[j] == (j != i as nat)
+      invariant forall j :: 0 <= j < |s2| ==> lseq_has(s2)[j] == (j != i)
       // Everything before i has its original value
-      invariant forall j :: 0 <= j <= i as nat - 1 ==> s2[j] == old(s)[j]
+      invariant forall j :: 0 <= j <= i - 1 ==> s2[j] == old(s)[j]
       // Everything after i has the value of its original -1 neighbor
-      invariant forall j :: i as nat +1 <= j < |s2| ==> s2[j] == old(s)[j-1]
+      invariant forall j :: i + 1 <= j < |s2| ==> s2[j] == old(s)[j-1]
     {
       linear var prevElt;
       s2, prevElt := lseq_take(s2, i-1);
